PCUICWcbvEvalCurrent.v
@@ -1,0 +1,276 @@
+(* Distributed under the terms of the MIT license.   *)
+(* Copied from the MetaCoq repo. Eventually, will be replced with the
+actual version from MetaCoq after making it compatible with Coq 8.10 *)
+Set Warnings "-notation-overridden".
+
+From Coq Require Import Bool String List Program BinPos Compare_dec Lia CRelationClasses.
+From Template Require Import config utils AstUtils.
+Import Template.BasicAst.
+From PCUIC Require Import PCUICAst PCUICAstUtils PCUICInduction PCUICLiftSubst PCUICUnivSubst PCUICTyping.
+Require Import String.
+Local Open Scope string_scope.
+Set Asymmetric Patterns.
+
+Set Asymmetric Patterns.
+Require Import ssreflect ssrbool.
+
+Local Ltac inv H := inversion H; subst.
+
+(** * Weak-head call-by-value evaluation strategy.
+  The [wcbveval] inductive relation specifies weak cbv evaluation.  It
+  is shown to be a subrelation of the 1-step reduction relation from
+  which conversion is defined. Hence two terms that reduce to the same
+  wcbv head normal form are convertible.
+  This reduction strategy is supposed to mimick at the Coq level the
+  reduction strategy of ML programming languages. It is used to state
+  the extraction conjecture that can be applied to Coq terms to produce
+  (untyped) terms where all proofs are erased to a dummy value. *)
+
+(** ** Big step version of weak cbv beta-zeta-iota-fix-delta reduction. *)
+
+Definition atom t :=
+  match t with
+  | tConstruct _ _ _
+  | tFix _ _
+  | tCoFix _ _
+  | tLambda _ _ _
+  | tSort _
+  | tProd _ _ _ => true
+  | _ => false
+  end.
+
+Definition isArityHead t :=
+  match t with
+  | tSort _
+  | tProd _ _ _ => true
+  | _ => false
+  end.
+
+Definition isEvar t :=
+  match t with
+  | tEvar _ _ => true
+  | _ => false
+  end.
+
+Definition isFix t :=
+  match t with
+  | tFix _ _ => true
+  | _ => false
+  end.
+
+Definition isFixApp t :=
+  match fst (decompose_app t) with
+  | tFix _ _ => true
+  | _ => false
+  end.
+
+Definition isCoFix t :=
+  match t with
+  | tCoFix _ _ => true
+  | _ => false
+  end.
+
+Definition isConstruct t :=
+  match t with
+  | tConstruct _ _ _ => true
+  | _ => false
+  end.
+
+Definition isAssRel Γ x :=
+  match x with
+  | tRel i =>
+    match option_map decl_body (nth_error Γ i) with
+    | Some None => true
+    | _ => false
+    end
+  | _ => false
+  end.
+
+Definition isAxiom Σ x :=
+  match x with
+  | tConst c u =>
+    match lookup_env Σ c with
+    | Some (ConstantDecl _ {| cst_body := None |}) => true
+    | _ => false
+    end
+  | _ => false
+  end.
+
+Definition isStuckFix t args :=
+  match t with
+  | tFix mfix idx =>
+    match unfold_fix mfix idx with
+    | Some (narg, fn) =>
+      ~~ is_constructor narg args
+    | None => false
+    end
+  | _ => false
+  end.
+
+Lemma atom_mkApps f l : atom (mkApps f l) -> (l = []) /\ atom f.
+Proof.
+  revert f; induction l using rev_ind. simpl. intuition auto.
+  simpl. intros. now rewrite -mkApps_nested in H.
+Qed.
+
+Section Wcbv.
+  Context (Σ : global_declarations) (Γ : context).
+  (* The local context is fixed: we are only doing weak reductions *)
+
+  Inductive eval : term -> term -> Prop :=
+  (** Reductions *)
+  (** Beta *)
+  | eval_beta f na t b a a' res :
+      eval f (tLambda na t b) ->
+      eval a a' ->
+      eval (subst10 a' b) res ->
+      eval (tApp f a) res
+
+  (** Let *)
+  | eval_zeta na b0 b0' t b1 res :
+      eval b0 b0' ->
+      eval (subst10 b0' b1) res ->
+      eval (tLetIn na b0 t b1) res
+
+  (** Local variables: defined or undefined *)
+  | eval_rel_def i body res :
+      option_map decl_body (nth_error Γ i) = Some (Some body) ->
+      eval (lift0 (S i) body) res ->
+      eval (tRel i) res
+
+  | eval_rel_undef i :
+      option_map decl_body (nth_error Γ i) = Some None ->
+      eval (tRel i) (tRel i)
+
+  (** Constant unfolding *)
+  | eval_delta c decl body (isdecl : declared_constant Σ c decl) u res :
+      decl.(cst_body) = Some body ->
+      eval (subst_instance_constr u body) res ->
+      eval (tConst c u) res
+
+  (** Axiom *)
+  | eval_axiom c decl (isdecl : declared_constant Σ c decl) u :
+      decl.(cst_body) = None ->
+      eval (tConst c u) (tConst c u)
+
+  (** Case *)
+  | eval_iota ind pars discr c u args p brs res :
+      eval discr (mkApps (tConstruct ind c u) args) ->
+      eval (iota_red pars c args brs) res ->
+      eval (tCase (ind, pars) p discr brs) res
+
+  (** Proj *)
+  | eval_proj i pars arg discr args k u a res :
+      eval discr (mkApps (tConstruct i k u) args) ->
+      nth_error args (pars + arg) = Some a ->
+      eval a res ->
+      eval (tProj (i, pars, arg) discr) res
+
+  (** Fix unfolding, with guard *)
+  | eval_fix f mfix idx args args' narg fn res :
+      eval f (tFix mfix idx) ->
+      unfold_fix mfix idx = Some (narg, fn) ->
+      (* There must be at least one argument for this to succeed *)
+      is_constructor narg args' ->
+      (** We unfold only a fix applied exactly to narg arguments,
+          avoiding overlap with [eval_beta] when there are more arguments. *)
+      S narg = #|args| ->
+      (* NOTE: we modify the ralation to match the traslation from Oak.
+         For the translated terms we always know that the fixpoint is defined by
+         recursion of the firts argument *)
+      narg = 0 ->
+      (* We reduce all arguments before unfolding *)
+      All2 eval args args' ->
+      eval (mkApps fn args') res ->
+      eval (mkApps f args) res
+
+  (** Fix stuck, with guard *)
+           (** We ignore this case, because it is not relevant for the Oak/Acorn translation *)
+  (* | eval_fix_value f mfix idx args args' : *)
+  (*     eval f (tFix mfix idx) -> *)
+  (*     (* We reduce all arguments to produce a suspended fix application value *)
+  (*        Note that the stuck fixpoint can be applied to any number of arguments *)
+  (*        here. *) *)
+  (*     All2 eval args args' -> *)
+  (*     isStuckFix (tFix mfix idx) args' -> *)
+  (*     eval (mkApps f args) (mkApps (tFix mfix idx) args') *)
+
+  (** CoFix-case unfolding *)
+  | red_cofix_case ip mfix idx p args narg fn brs res :
+      unfold_cofix mfix idx = Some (narg, fn) ->
+      eval (tCase ip p (mkApps fn args) brs) res ->
+      eval (tCase ip p (mkApps (tCoFix mfix idx) args) brs) res
+
+  (** CoFix-proj unfolding *)
+  | red_cofix_proj p mfix idx args narg fn res :
+      unfold_cofix mfix idx = Some (narg, fn) ->
+      eval (tProj p (mkApps fn args)) res ->
+      eval (tProj p (mkApps (tCoFix mfix idx) args)) res
+
+  (** Non redex-producing heads applied to values are values *)
+  | eval_app_cong f f' a a' :
+      eval f f' ->
+      ~~ (isLambda f' || isFixApp f' || isArityHead f') ->
+      eval a a' ->
+      eval (tApp f a) (tApp f' a')
+
+  (** Evars complicate reasoning due to the embedded substitution, we skip
+      them for now *)
+  (* | eval_evar n l l' : *)
+  (*     Forall2 eval l l' -> *)
+  (*     eval (tEvar n l) (tEvar n l') *)
+
+
+  (** Atoms are values (includes abstractions, cofixpoints and constructors
+      along with type constructors) *)
+  | eval_atom t : atom t -> eval t t.
+
+  (** Characterization of values for this reduction relation.
+      Only constructors and cofixpoints can accumulate arguments.
+      All other values are atoms and cannot have arguments:
+      - box
+      - abstractions
+      - constant constructors
+      - unapplied fixpoints and cofixpoints
+   *)
+
+  Definition value_head x :=
+    isConstruct x || isCoFix x || isAssRel Γ x || isAxiom Σ x.
+
+  (* Lemma value_head_atom x : value_head x -> atom x. *)
+  (* Proof. destruct x; auto. Qed. *)
+
+  Inductive value : term -> Prop :=
+  | value_atom t : atom t -> value t
+  (* | value_evar n l l' : Forall value l -> Forall value l' -> value (mkApps (tEvar n l) l') *)
+  | value_app t l : value_head t -> All value l -> value (mkApps t l)
+  | value_stuck_fix f args :
+      All value args ->
+      isStuckFix f args ->
+      value (mkApps f args)
+  .
+
+  (* Lemma value_values_ind : forall P : term -> Prop, *)
+  (*     (forall t, atom t -> P t) -> *)
+  (*     (* (forall n l l', Forall value l -> Forall P l -> Forall value l' -> Forall P l' -> *) *)
+  (*     (*                 P (mkApps (tEvar n l) l')) -> *) *)
+  (*     (forall t l, value_head t -> All value l -> All P l -> P (mkApps t l)) -> *)
+  (*     (forall f args, *)
+  (*         All value args -> *)
+  (*         All P args -> *)
+  (*         isStuckFix f args -> *)
+  (*         P (mkApps f args)) -> *)
+  (*     forall t : term, value t -> P t. *)
+  (* Proof. *)
+  (*   intros P ???. *)
+  (*   fix value_values_ind 2. destruct 1. *)
+  (*   - easy. *)
+  (*   - eapply H0; auto. *)
+  (*     revert l a. fix aux 2. destruct 1. constructor; auto. *)
+  (*     constructor. now eapply value_values_ind. now apply aux. *)
+  (*   - eapply X1; eauto. *)
+  (*     clear i. revert args a. fix aux 2. destruct 1. constructor; auto. *)
+  (*     constructor. now eapply value_values_ind. now apply aux. *)
+  (* Defined. *)
+
+  End Wcbv.
